another refactor

Diploma/Order/MonomialOrder.lean
@@ -13,46 +13,54 @@ class MonomialOrder (α : Type u) [HMul α α α] extends LinearOrder α :=
  add_le_add : ∀ a b c: α, a < b → a * c < b * c
 
 --# Lex order
---# a <_lex b ↔ ∃ c: a = c ++ p₁, b = c ++ p₂ ∧ p₁[0] < p₂[0]
+--# a <=_lex b ↔ ∃ c: a = c ++ p₁, b = c ++ p₂ ∧ p₁[0] < p₂[0]
 def Order.lex_impl (v₁ v₂ : Vector Nat n): Prop :=
   match v₁, v₂ with
-    | ⟨[], _⟩  , ⟨[], _⟩   => False
+    | ⟨[], _⟩  , ⟨[], _⟩   => True
     | ⟨x::_, _⟩, ⟨y::_, _⟩ => if x = y then lex_impl v₁.tail v₂.tail 
-                              else x < y
+                              else x ≤ y
 
 def Order.lex (v₁ v₂ : Variables n order.Lex): Prop := Order.lex_impl v₁ v₂
 
-def Order.lex_le (v₁ v₂ : Variables n order.Lex): Prop := if v₁ = v₂ then True
-                                                          else Order.lex v₁ v₂  
-
-private def Order.blt_lex_impl (v₁ v₂ : Vector Nat n): Bool :=
+private def Order.ble_lex_impl (v₁ v₂ : Vector Nat n): Bool :=
   match v₁, v₂ with
-    | ⟨[], _⟩  , ⟨[], _⟩   => false
-    | ⟨x::_, _⟩, ⟨y::_, _⟩ => if x == y then blt_lex_impl v₁.tail v₂.tail 
-                              else x < y
-
-private def Order.ble_lex_impl (v₁ v₂ : Vector Nat n): Bool := v₁ == v₂ ∨ Order.blt_lex_impl v₁ v₂  
+    | ⟨[], _⟩  , ⟨[], _⟩   => true
+    | ⟨x::_, _⟩, ⟨y::_, _⟩ => if x == y then ble_lex_impl v₁.tail v₂.tail 
+                              else x ≤ y
 
 --# Ordering theorems
-theorem lex_le_refl : ∀ (a : Variables n order.Lex), Order.lex_le a a := by
+theorem lex_le_refl : ∀ (a : Variables n order.Lex), Order.lex a a := by
   intro a
-  match a with 
-    | ⟨[], p⟩    => rw [Order.lex_le]
-                    simp                          
-    | ⟨x::xs, _⟩ => rw [Order.lex_le, Order.lex, Order.lex_impl]
-                    split
-                    simp
-                    simp at *
+  let rec aux (m: Nat) (v: Variables m order.Lex) : Order.lex_impl v v := by 
+    match v with 
+      | ⟨[], p⟩    => rw [Order.lex_impl]
+                      split
+                      simp at *
+                      simp at p
+                      simp at *                                   
+      | ⟨x::xs, _⟩ => rw [Order.lex_impl]
+                      split
+                      simp
+                      simp at *
+                      simp at *
+                      simp [Nat.le_refl]
+                      rename_i x₁ _ x₂ _ h₁ h₂
+                      have h₃ := Eq.symm h₁.left
+                      have h₄ := Eq.symm h₂.left
+                      rw [h₃, h₄]
+                      simp [Nat.le_refl]
+                      apply aux (m-1) (tail ⟨x::xs, _⟩)
+  exact aux n a
 
-theorem lex_lt_trans (a b c : Variables n order.Lex): Order.lex a b → Order.lex b c → Order.lex a c := by
-  intros h₁ h₂
+theorem lex_le_trans : ∀ (a b c : Variables n order.Lex), Order.lex a b → Order.lex b c → Order.lex a c := by
+  intros v₁ v₂ v₃ h₁ h₂
   let rec aux (m: Nat) (a b c: Variables m order.Lex) 
               (ab : Order.lex_impl a b) (bc : Order.lex_impl b c) : Order.lex_impl a c := by 
     match a, b, c with
-      | ⟨[], p⟩,    ⟨[], q⟩,    ⟨[], l⟩    => rw [Order.lex_impl] at ab bc
-                                              split at ab 
-                                              split at bc
-                                              repeat contradiction
+      | ⟨[], p⟩,    ⟨[], q⟩,    ⟨[], l⟩    => rw [Order.lex_impl]
+                                              split
+                                              simp
+                                              simp at *
       | ⟨x::xs, p⟩, ⟨y::ys, q⟩, ⟨z::zs, l⟩ => rw [Order.lex_impl] 
                                               rw [Order.lex_impl] at ab bc
                                               split at ab
@@ -104,7 +112,7 @@ theorem lex_lt_trans (a b c : Variables n order.Lex): Order.lex a b → Order.le
                                               rw [x_cross_eq_x, y_cross_eq_x] at neq₂ bc
                                               rw [x_cross_one_eq_x, y_cross_one_eq_y] at neq₁ ab
                                               rw [eq₁] at ab
-                                              have eq_eq := Nat.lt_asymm bc ab
+                                              have eq_eq := Nat.le_antisymm bc ab
                                               contradiction 
                                               split at ab
                                               split at bc
@@ -146,41 +154,15 @@ theorem lex_lt_trans (a b c : Variables n order.Lex): Order.lex a b → Order.le
                                               rename_i neq₃
                                               rw [x_cross_one_eq_x, y_cross_one_eq_y] at neq₂ ab
                                               rw [x_cross_eq_x, y_cross_eq_x] at neq₃ bc
-                                              have le_le := Nat.lt_trans ab bc
+                                              have le_le := Nat.le_trans ab bc
                                               exact le_le                        
-  exact aux n a b c h₁ h₂
+  exact aux n v₁ v₂ v₃ h₁ h₂
 
-theorem lex_le_trans : ∀ (a b c : Variables n order.Lex), Order.lex_le a b → Order.lex_le b c → Order.lex_le a c := 
-  by
-    intros a b c ab bc
-    rw [Order.lex_le]
-    rw [Order.lex_le] at ab bc
-    split at ab
-    split at bc
-    rename_i eq₁ eq₂
-    rw [eq₂] at eq₁
-    simp [eq₁]
-    rename_i eq leq
-    rw [←eq] at leq
-    simp [leq]
-    rw [←eq] at bc
-    exact bc
-    split at bc
-    rename_i neq eq
-    rw [eq] at neq
-    split
-    simp
-    rw [eq] at ab
-    exact ab
-    split
-    simp
-    exact lex_lt_trans a b c ab bc 
-
-theorem lex_lt_antisymm : ∀ (a b : Variables n order.Lex), Order.lex a b → Order.lex b a → a = b := by
+theorem lex_le_antisymm : ∀ (a b : Variables n order.Lex), Order.lex a b → Order.lex b a → a = b := by
   intros v₁ v₂ h₁ h₂
   let rec aux (m: Nat) (a b: Vector Nat m) (ab: Order.lex_impl a b) (ba: Order.lex_impl b a): a = b := by 
     match a, b with
-      | ⟨[], p⟩, ⟨[], _⟩       => simp 
+      | ⟨[], p⟩, ⟨[], q⟩       => simp 
       | ⟨x::xs, p⟩, ⟨y::ys, q⟩ => rw [Order.lex_impl] at ab ba
                                   simp at *
                                   split at ab
@@ -200,85 +182,54 @@ theorem lex_lt_antisymm : ∀ (a b : Variables n order.Lex), Order.lex a b → O
                                   have eq_symm := Eq.symm eq
                                   contradiction
                                   rename_i neq₁ neq₂
-                                  have eq := Nat.lt_asymm ab ba
+                                  have eq := Nat.le_antisymm ab ba
                                   contradiction
-  exact aux n v₁ v₂ h₁ h₂ 
+  exact aux n v₁ v₂ h₁ h₂ theorem vectors_neq_r_head_neq (v₁ v₂: Vector Nat (Nat.succ n)) (h: v₁ ≠ v₂): head v₁ ≠ head v₂ := by sorry 
 
-theorem lex_le_antisymm : ∀ (a b : Variables n order.Lex), Order.lex_le a b → Order.lex_le b a → a = b := by
-  intros a b le₁ le₂
-  rw [Order.lex_le] at le₁ le₂
-  split at le₁
-  split at le₂
-  rename_i h
-  rw [h] 
-  rename_i h _
-  exact h
-  split at le₂
-  rename_i h
-  simp [h]
-  exact lex_lt_antisymm a b le₁ le₂  
-
-theorem vectors_neq_r_head_neq (v₁ v₂: Vector Nat (Nat.succ n)) (h: v₁ ≠ v₂): head v₁ ≠ head v₂ := by sorry 
-
-theorem lex_lt_semi_total (v₁ v₂ : Variables n order.Lex) (not_eq: v₁ ≠ v₂): Order.lex v₁ v₂ ∨ Order.lex v₂ v₁ := by
-  let rec aux (m: Nat) (a b: Vector Nat m) (not_eq_: a ≠ b): (Order.lex_impl a b ∨ Order.lex_impl b a) := by
+theorem lex_le_total : ∀ (a b : Variables n order.Lex), Order.lex a b ∨ Order.lex b a := by
+  intros v₁ v₂
+  let rec aux (m: Nat) (a b: Vector Nat m) : Order.lex_impl a b ∨ Order.lex_impl b a := by
     match a, b with
-      | ⟨[], p⟩, ⟨[], q⟩       => simp at not_eq_
-      | ⟨x::xs, p⟩, ⟨y::ys, q⟩ => rw [Order.lex_impl]
-                                  split
-                                  rw [Order.lex_impl]
+      | ⟨[], p⟩, ⟨[], q⟩       => rw [Order.lex_impl]
                                   split
                                   simp
                                   simp at *
+      | ⟨x::xs, p⟩, ⟨y::ys, q⟩ => rw [Order.lex_impl]
+                                  simp [Or.comm]
+                                  rw [Order.lex_impl]
+                                  split
+                                  simp
+                                  split
+                                  split
+                                  simp [Or.comm]
+                                  apply aux (m-1) (tail ⟨x::xs, p⟩) (tail ⟨y::ys, q⟩)
+                                  simp at *
+                                  rename_i eq neq heq₁ heq₂
+                                  have s_eq := Eq.symm eq
+                                  have eq_1 := Eq.symm heq₁.left
+                                  have eq_2 := Eq.symm heq₂.left
+                                  rw [eq_1, eq_2] at s_eq
+                                  contradiction
                                   split
                                   simp at *
+                                  rename_i neq eq heq₁ heq₂
+                                  have s_eq := Eq.symm eq
+                                  have eq_1 := heq₁.left
+                                  have eq_2 := heq₂.left
+                                  rw [eq_1, eq_2] at s_eq
+                                  contradiction
                                   simp at *
-                                  split
-                                  simp at *
-                                  rename_i eq ceq₁ ceq₂
-                                  have eq₁ := ceq₁.left
-                                  have eq₂ := ceq₂.left
-                                  rw [← eq₁, ←eq₂] at eq
-                                  sorry
-                                  sorry
-                                  -- rename_i eq neq heq₁ heq₂
-                                  -- have s_eq := Eq.symm eq
-                                  -- have eq_1 := Eq.symm heq₁.left
-                                  -- have eq_2 := Eq.symm heq₂.left
-                                  -- rw [eq_1, eq_2] at s_eq
-                                  -- contradiction
-                                  -- split
-                                  -- simp at *
-                                  -- rename_i neq eq heq₁ heq₂
-                                  -- have s_eq := Eq.symm eq
-                                  -- have eq_1 := heq₁.left
-                                  -- have eq_2 := heq₂.left
-                                  -- rw [eq_1, eq_2] at s_eq
-                                  -- contradiction
-                                  -- simp at *
-                                  -- rename_i r _ heq₁ heq₂
-                                  -- have eq_1 := heq₁.left
-                                  -- have eq_2 := heq₂.left
-                                  -- rw [eq_1, eq_2]
-                                  -- simp [Nat.le_total]
-                                  -- exact r
-  exact aux n v₁ v₂ not_eq
-  
-theorem lex_le_total : ∀ (a b : Variables n order.Lex), Order.lex_le a b ∨ Order.lex_le b a := by 
-  intros a b
-  rw [Order.lex_le, Order.lex_le]
-  split
-  split
-  simp; simp
-  split
-  simp
-  rename_i h _
-  simp [lex_lt_semi_total, h] 
+                                  rename_i heq₁ heq₂
+                                  have eq_1 := heq₁.left
+                                  have eq_2 := heq₂.left
+                                  rw [eq_1, eq_2]
+                                  simp [Nat.le_total]
+  exact aux n v₁ v₂
 
-theorem lex_lt_iff_le_not_le: ∀ (a b : Variables n order.Lex), Order.lex a b ↔ Order.lex_le a b ∧ ¬ Order.lex_le b a := by
+theorem lex_lt_iff_le_not_le: ∀ (a b : Variables n order.Lex), Order.lex a b ↔ Order.lex a b ∧ ¬ Order.lex b a := by
   sorry
   
-theorem lex_add_lt_add : ∀ a b c: Variables n order.Lex, Order.lex a b → Order.lex (Variables.mul a c) (Variables.mul b c) := by
+theorem lex_add_le_add : ∀ a b c: Variables n order.Lex, Order.lex a b → Order.lex (Variables.mul a c) (Variables.mul b c) := by
   intros v₁ v₂ v₃
   let rec aux (m: Nat) (a b c: Variables m order.Lex) : Order.lex_impl a b → Order.lex_impl (Variables.mul a c) (Variables.mul b c) := by
    intros h 
@@ -286,86 +237,64 @@ theorem lex_add_lt_add : ∀ a b c: Variables n order.Lex, Order.lex a b → Ord
     | ⟨[], _⟩, ⟨[], _⟩, ⟨[], _⟩          => rw [Order.lex_impl]
                                             split
                                             simp
-                                            sorry
-                                            sorry
+                                            split
                                             repeat (rename_i prop₁ _ _ _ _ _ _ _ _ _ prop₄ _ _ _
                                                     simp at prop₁ prop₄
                                                     simp [Eq.symm prop₁] at prop₄)                                                                                  
     | ⟨x::xs, p₁⟩, ⟨y::ys, p₂⟩, ⟨z::zs, p₃⟩ => rw [Order.lex_impl]
                                                split
                                                simp
-                                               sorry
-                                               sorry
-                                               --split
-                                               --apply aux (m-1) (tail ⟨x::xs, p₁⟩) (tail ⟨y::ys, p₂⟩) (tail ⟨z::zs, p₃⟩)
-                                               --rw [Order.lex_impl] at h
-                                               --split at h
-                                               --rename_i prop₁ _ _ _ _ _ _ prop₂ _ _
-                                               --simp at prop₁ prop₂
-                                               --simp [Eq.symm prop₂] at prop₁
-                                               --split at h
-                                               --exact h
-                                               --simp at *
-                                               --rename_i var_mul₁ var_mul₂ _ _ _ _ _ _ _ _ eq neq heq₁ heq₂
-                                               --simp [map₂, Variables.mul, List.zipWith] at var_mul₁ var_mul₂
-                                               --have eq₁ := heq₁.left 
-                                               --have eq₂ := heq₂.left
-                                               --cases var_mul₁
-                                               --cases var_mul₂
-                                               --rename_i sum_eq _
-                                               --simp [eq₁, eq₂] at sum_eq
-                                               --contradiction
-                                               --rw [Order.lex_impl] at h
-                                               --split at h
-                                               --simp at *
-                                               --split at h
-                                               --rename_i var_mul₁ var_mul₂ _ _ _ _ _ _ _ _ _ heq₁ heq₂ eq
-                                               --simp [map₂, Variables.mul, List.zipWith] at var_mul₁ var_mul₂
-                                               --cases heq₁
-                                               --cases heq₂
-                                               --cases var_mul₁
-                                               --cases var_mul₂
-                                               --simp [eq]
-                                               --rename_i eq _ _ hneq₂ _
-                                               --simp at *
-                                               --contradiction
-                                               --rename_i var_mul₁ var_mul₂ _ _ _ _ _ _ _ _ _ heq₁ heq₂ neq
-                                               --cases heq₁
-                                               --cases heq₂
-                                               --cases var_mul₁
-                                               --cases var_mul₂
-                                               --simp
-                                               --exact h
+                                               split
+                                               apply aux (m-1) (tail ⟨x::xs, p₁⟩) (tail ⟨y::ys, p₂⟩) (tail ⟨z::zs, p₃⟩)
+                                               rw [Order.lex_impl] at h
+                                               split at h
+                                               rename_i prop₁ _ _ _ _ _ _ prop₂ _ _
+                                               simp at prop₁ prop₂
+                                               simp [Eq.symm prop₂] at prop₁
+                                               split at h
+                                               exact h
+                                               simp at *
+                                               rename_i var_mul₁ var_mul₂ _ _ _ _ _ _ _ _ eq neq heq₁ heq₂
+                                               simp [map₂, Variables.mul, List.zipWith] at var_mul₁ var_mul₂
+                                               have eq₁ := heq₁.left 
+                                               have eq₂ := heq₂.left
+                                               cases var_mul₁
+                                               cases var_mul₂
+                                               rename_i sum_eq _
+                                               simp [eq₁, eq₂] at sum_eq
+                                               contradiction
+                                               rw [Order.lex_impl] at h
+                                               split at h
+                                               simp at *
+                                               split at h
+                                               rename_i var_mul₁ var_mul₂ _ _ _ _ _ _ _ _ _ heq₁ heq₂ eq
+                                               simp [map₂, Variables.mul, List.zipWith] at var_mul₁ var_mul₂
+                                               cases heq₁
+                                               cases heq₂
+                                               cases var_mul₁
+                                               cases var_mul₂
+                                               simp [eq]
+                                               rename_i var_mul₁ var_mul₂ _ _ _ _ _ _ _ _ _ heq₁ heq₂ eq
+                                               cases heq₁
+                                               cases heq₂
+                                               simp [map₂, Variables.mul, List.zipWith] at var_mul₁ var_mul₂
+                                               cases var_mul₁ 
+                                               cases var_mul₂
+                                               simp at *
+                                               exact h
   apply aux n v₁ v₂ v₃
 
 --# Decidable theorems
-theorem lex_true_of_blt_lex_true (h: Eq (Order.blt_lex_impl v₁ v₂) true): Order.lex v₁ v₂ := by
-  let rec aux (m: Nat) (a b: Vector Nat m) (h: Eq (Order.blt_lex_impl a b) true): Order.lex a b := by
+theorem Order.lex_true_of_ble_lex_true (h: Eq (Order.ble_lex_impl v₁ v₂) true): Order.lex v₁ v₂ := by
+  let rec aux (m: Nat) (a b: Vector Nat m) (h: Eq (Order.ble_lex_impl a b) true): Order.lex a b := by
     rw [Order.lex]
     rw [Order.lex_impl]
     match a, b with
-      | ⟨[], _⟩  , ⟨[], _⟩     => rw [Order.blt_lex_impl] at h
-                                  split at h
-                                  simp at *
-                                  split
-                                  rename_i heq _ _
-                                  simp at heq
-                                  rename_i heq _ _
-                                  simp at heq
+      | ⟨[], _⟩  , ⟨[], _⟩     => simp
       | ⟨x::xs, _⟩, ⟨y::ys, _⟩ => split
-                                  rw [Order.blt_lex_impl] at h
-                                  split at h
-                                  simp at h
-                                  rename_i heq₁ heq₂ _ _ _ _ _ _ _ _ heq₃ heq₄ 
-                                  split at h
-                                  rw [heq₁] at heq₃ 
-                                  rw [heq₂] at heq₄
-                                  rename_i heq
-                                  sorry
-                                  sorry
                                   simp
                                   split
-                                  rw [Order.blt_lex_impl] at h
+                                  rw [Order.ble_lex_impl] at h
                                   simp at h
                                   split at h
                                   exact aux (m-1) (tail ⟨x::xs, _⟩) (tail ⟨y::ys, _⟩) h
@@ -376,7 +305,7 @@ theorem lex_true_of_blt_lex_true (h: Eq (Order.blt_lex_impl v₁ v₂) true): Or
                                   rw [eq₁, eq₂] at hneq
                                   contradiction                                  
                                   rename_i heq₁ heq₂ hneq₁ 
-                                  rw [Order.blt_lex_impl] at h
+                                  rw [Order.ble_lex_impl] at h
                                   split at h
                                   simp at *
                                   split at h
@@ -404,55 +333,51 @@ theorem lex_true_of_blt_lex_true (h: Eq (Order.blt_lex_impl v₁ v₂) true): Or
   rename_i n
   exact aux n v₁ v₂ h                                 
 
-theorem lex_le_true_of_blt_lex_true (h: Eq (Order.blt_lex_impl v₁ v₂) true): Order.lex_le v₁ v₂ := by 
-  rw [Order.lex_le]
-  split
-  simp
-  simp [lex_true_of_blt_lex_true, h]
-
-theorem blt_eq_true_of_lex_le (h: Order.lex_le v₁ v₂) : Eq (Order.ble_lex_impl v₁ v₂) true := by
-  let rec aux (m: Nat) (a b: Vector Nat m) (h: Order.lex_le a b): Eq (Order.ble_lex_impl a b) true := by 
+theorem Order.ble_eq_true_of_lex (h: Order.lex_impl v₁ v₂) : Eq (Order.ble_lex_impl v₁ v₂) true := by
+  let rec aux (m: Nat) (a b: Vector Nat m) (h: Order.lex_impl a b): Eq (Order.ble_lex_impl a b) true := by 
      match a, b with
-      | ⟨[], _⟩, ⟨[], _⟩       => rw [Order.lex_le] at h
-                                  split at h
-                                  rw [Order.ble_lex_impl]
-                                  simp
-                                  simp at *
-      | ⟨x::xs, _⟩, ⟨y::ys, _⟩ => rw [Order.lex_le] at h
-                                  split at h
-                                  rw [Order.ble_lex_impl, algebra.Order.blt_lex_impl]
-                                  simp
-                                  rename_i heq 
+      | ⟨[], _⟩, ⟨[], _⟩       => rw [Order.ble_lex_impl]
+      | ⟨x::xs, _⟩, ⟨y::ys, _⟩ => rw [Order.ble_lex_impl]
+                                  split;rfl
                                   split
-                                  simp [heq]
-                                  cases heq
-                                  simp
-                                  rw [Order.lex, Order.lex_impl] at h
-                                  rw [Order.ble_lex_impl, algebra.Order.blt_lex_impl]
+                                  rw [lex_impl] at h
+                                  simp at h
                                   split at h
-                                  simp at *
+                                  apply Order.ble_eq_true_of_lex h
+                                  rename_i heq₁ heq₂ neq eq
+                                  simp at heq₁ heq₂
+                                  have eq₁ := heq₁.left
+                                  have eq₂ := heq₂.left
+                                  simp at neq
+                                  rw [eq₁, eq₂] at eq
+                                  contradiction
+                                  rw [lex_impl] at h
+                                  simp at h
                                   split at h
-                                  simp at *
+                                  rename_i heq₁ heq₂ neq eq
+                                  simp at heq₁ heq₂
+                                  have eq₁ := heq₁.left
+                                  have eq₂ := heq₂.left
+                                  simp at neq
+                                  rw [eq₁, eq₂] at eq
+                                  contradiction
                                   simp
-                                  split
-                                  sorry
-                                  sorry
-                                  sorry
+                                  rename_i heq₁ heq₂ _ _
+                                  simp at heq₁ heq₂
+                                  have eq₁ := Eq.symm heq₁.left
+                                  have eq₂ := Eq.symm heq₂.left
+                                  rwa [eq₁, eq₂]
   rename_i n
   exact aux n v₁ v₂ h 
 
-theorem lex_le_false_of_blt_lex_false (h: Not (Eq (Order.ble_lex_impl v₁ v₂) true)): Not (Order.lex_le v₁ v₂) :=  
-  fun h' => absurd (blt_eq_true_of_lex_le h') h
+theorem Order.lex_false_of_ble_lex_false (h: Not (Eq (Order.ble_lex_impl v₁ v₂) true)): Not (Order.lex v₁ v₂) :=
+  fun h' => absurd (Order.ble_eq_true_of_lex h') h
 
-
-instance Order.lex_decidable (v₁ v₂: Variables n order.Lex): Decidable (Order.lex_le v₁ v₂) :=
-  dite (Eq (Order.blt_lex_impl v₁ v₂) true) (fun h => isTrue (lex_le_true_of_blt_lex_true h))
-                                            (fun h => isFalse (lex_le_false_of_blt_lex_false h))
-
-
+instance Order.lex_decidable (v₁ v₂: Variables n order.Lex): Decidable (Order.lex v₁ v₂) :=
+  dite (Eq (Order.ble_lex_impl v₁ v₂) true) (fun h => isTrue (Order.lex_true_of_ble_lex_true h))
+                                            (fun h => isFalse (Order.lex_false_of_ble_lex_false h))
 --# Grlex order
---# a <_grlex b ↔ |a| < |b| ∨ |a| = |b| ∧ a <_lex b 
-
+--# a <=_grlex b ↔ |a| < |b| ∨ |a| = |b| ∧ a <_lex b 
 def Order.grlex (vs₁ vs₂: Variables n order.GrLex): Prop :=
   let sum₁ := elem_sum vs₁ 
   let sum₂ := elem_sum vs₂   
@@ -463,37 +388,30 @@ def Order.grlex (vs₁ vs₂: Variables n order.GrLex): Prop :=
     elem_sum (vs: Variables n order.GrLex): Nat :=
       List.foldl (fun x y => x + y) 0 vs.toList
 
-def Order.grlex_le (v₁ v₂ : Variables n order.GrLex): Prop := v₁ = v₂ ∨ Order.grlex v₁ v₂ 
-
 private def Order.bgrlex (vs₁ vs₂: Variables n order.GrLex): Bool :=
   let sum₁ := elem_sum vs₁ 
   let sum₂ := elem_sum vs₂   
   if sum₁ < sum₂ then true
-  else if sum₁ = sum₂ then Order.blt_lex_impl vs₁ vs₂
+  else if sum₁ = sum₂ then Order.lex vs₁ vs₂
   else false
   where
     elem_sum (vs: Variables n order.GrLex): Nat :=
-      List.foldl (fun x y => x + y) 0 vs.toList 
+      List.foldl (fun x y => x + y) 0 vs.toList
 
 --# Ordering theorems
-theorem grlex_lt_iff_le_not_le : ∀ (a b : Variables n order.GrLex), Order.grlex a b ↔ Order.grlex_le a b ∧ ¬Order.grlex_le b a := 
+theorem grlex_lt_iff_le_not_le : ∀ (a b : Variables n order.GrLex), Order.grlex a b ↔ Order.grlex a b ∧ ¬Order.grlex b a := 
   by 
     intros a b 
     apply Iff.intro
     sorry
     sorry
 
-theorem grlex_lt_refl: ∀ (a : Variables n order.GrLex), Order.grlex a a := by 
+theorem grlex_le_refl: ∀ (a : Variables n order.GrLex), Order.grlex a a := by 
   intros a
   simp [Order.grlex]
-  sorry
+  apply lex_le_refl
 
-theorem grlex_le_refl: ∀ (a : Variables n order.GrLex), Order.grlex_le a a := by
-  intros a
-  rw [Order.grlex_le]
-  simp
-
-theorem grlex_lt_trans : ∀ (a b c : Variables n order.GrLex), Order.grlex a b → Order.grlex b c → Order.grlex a c := by
+theorem grlex_le_trans : ∀ (a b c : Variables n order.GrLex), Order.grlex a b → Order.grlex b c → Order.grlex a c := by
   intros a b c ab bc
   simp [Order.grlex]
   simp [Order.grlex] at ab bc
@@ -524,7 +442,7 @@ theorem grlex_lt_trans : ∀ (a b c : Variables n order.GrLex), Order.grlex a b 
   split at bc
   rename_i nleq₁ nleq₂ eq₁ eq₂ neq₁ eq₃
   simp at *
-  apply lex_lt_trans
+  apply lex_le_trans
   exact ab
   exact bc
   repeat contradiction
@@ -536,27 +454,7 @@ theorem grlex_lt_trans : ∀ (a b c : Variables n order.GrLex), Order.grlex a b 
   rw [eq₁] at neq
   repeat contradiction
 
-theorem grlex_le_trans : ∀ (a b c : Variables n order.GrLex), Order.grlex_le a b → Order.grlex_le b c → Order.grlex_le a c := by
-  intros a b c ab bc
-  rw [Order.grlex_le]
-  rw [Order.grlex_le] at ab bc
-  cases ab
-  cases bc
-  rename_i h₁ h₂
-  rw [h₂] at h₁
-  simp [h₁]
-  rename_i h₁ h₂
-  rw [←h₁] at h₂
-  simp [h₂]
-  cases bc
-  rename_i h₁ h₂
-  rw [h₂] at h₁
-  simp [h₁]
-  rename_i h₁ h₂
-  apply Or.inr
-  apply grlex_lt_trans a b c h₁ h₂ 
-
-theorem grlex_lt_antisymm : ∀ (a b : Variables n order.GrLex), Order.grlex a b → Order.grlex b a → a = b := by 
+theorem grlex_le_antisymm : ∀ (a b : Variables n order.GrLex), Order.grlex a b → Order.grlex b a → a = b := by 
   intros a b ab ba
   simp [Order.grlex] at ab ba
   split at ab
@@ -576,40 +474,17 @@ theorem grlex_lt_antisymm : ∀ (a b : Variables n order.GrLex), Order.grlex a b
   rw [symm] at leq
   simp at leq
   split at ba
-  apply lex_lt_antisymm 
+  apply lex_le_antisymm 
   exact ab
   exact ba
   repeat contradiction
 
-theorem grlex_le_antisymm : ∀ (a b : Variables n order.GrLex), Order.grlex a b → Order.grlex b a → a = b := by 
-  intros a b h₁ h₂
-  rw [Order.grlex] at h₁ h₂
-  simp at h₁ h₂
-  split at h₁ 
-  split at h₂
-  rename_i lt₁
-  have not_lt := Nat.lt_asymm lt₁
-  contradiction
-  split at h₂
-  rename_i lt₁ nlt₂ eq
-  rw [←eq] at lt₁ nlt₂
-  simp at *
-  contradiction
-  split at h₁
-  split at h₂
-  rename_i nlt eq lt
-  rw [eq] at lt nlt
-  contradiction
-  split at h₂
-  apply lex_lt_antisymm a b h₁ h₂
-  repeat contradiction
-
-theorem grlex_lt_total : ∀ (a b : Variables n order.GrLex), Order.grlex a b ∨ Order.grlex b a := by 
+theorem grlex_le_total : ∀ (a b : Variables n order.GrLex), Order.grlex a b ∨ Order.grlex b a := by 
   intros a b
   simp [Order.grlex]
   split <;> simp
   split <;> repeat (first | split | simp)
-  sorry
+  simp [lex_le_total] 
   rename_i nleq₁ eq nleq₂ neq
   have contr := Eq.symm eq 
   contradiction
@@ -621,13 +496,7 @@ theorem grlex_lt_total : ∀ (a b : Variables n order.GrLex), Order.grlex a b �
   simp at *
   have contr := Nat.le_antisymm nleq₁ nleq₂
   contradiction
-
-theorem grlex_le_total : ∀ (a b : Variables n order.GrLex), Order.grlex_le a b ∨ Order.grlex_le b a := by 
-  intros a b 
-  rw [Order.grlex_le, Order.grlex_le]
-  rw [or_or_or_comm]
-  simp [grlex_lt_total]
-
+  
 theorem grlex_add_lt_add : ∀ a b c: Variables n order.GrLex, Order.grlex a b → Order.grlex (Variables.mul a c) (Variables.mul b c) := by
   intros v₁ v₂ v₃
   let rec aux (m: Nat) (a b c: Variables m order.GrLex) : Order.grlex a b → Order.grlex (Variables.mul a c) (Variables.mul b c) := by
@@ -638,7 +507,7 @@ theorem grlex_add_lt_add : ∀ a b c: Variables n order.GrLex, Order.grlex a b �
   exact aux n v₁ v₂ v₃ 
 
 --# Decidable theorems
-theorem grlex_true_of_blt_grlex_true (h: Eq (Order.bgrlex v₁ v₂) true): Order.grlex v₁ v₂ := by
+theorem grlex_true_of_ble_grlex_true (h: Eq (Order.bgrlex v₁ v₂) true): Order.grlex v₁ v₂ := by
   simp [Order.grlex]
   split
   simp
@@ -661,7 +530,7 @@ theorem grlex_true_of_blt_grlex_true (h: Eq (Order.bgrlex v₁ v₂) true): Orde
   have leq := Nat.le_of_not_lt nleq
   exact h leq
 
-theorem grblt_eq_true_of_grlex (h: Order.grlex v₁ v₂): Eq (Order.bgrlex v₁ v₂) true := by
+theorem grble_eq_true_of_grlex (h: Order.grlex v₁ v₂): Eq (Order.bgrlex v₁ v₂) true := by
   simp [Order.grlex] at h
   split at h
   simp [algebra.Order.bgrlex]
@@ -690,11 +559,11 @@ theorem grblt_eq_true_of_grlex (h: Order.grlex v₁ v₂): Eq (Order.bgrlex v₁
   rw [algebra.Order.bgrlex.elem_sum, algebra.Order.bgrlex.elem_sum] at le neq
   repeat contradiction
 
-theorem grlex_false_of_blt_grlex_false (h: Not (Eq (Order.bgrlex v₁ v₂) true)): Not (Order.grlex v₁ v₂) := 
-  fun h' => absurd (grblt_eq_true_of_grlex h') h
+theorem grlex_false_of_ble_grlex_false (h: Not (Eq (Order.bgrlex v₁ v₂) true)): Not (Order.grlex v₁ v₂) := 
+  fun h' => absurd (grble_eq_true_of_grlex h') h
   
-instance grlex_decidable (v₁ v₂: Variables n order.GrLex): Decidable (Order.grlex v₁ v₂) := 
-  dite (Eq (Order.bgrlex v₁ v₂) true) (fun h => isTrue (grlex_true_of_blt_grlex_true h))
-                                      (fun h => isFalse (grlex_false_of_blt_grlex_false h))
+instance Order.grlex_decidable (v₁ v₂: Variables n order.GrLex): Decidable (Order.grlex v₁ v₂) := 
+  dite (Eq (Order.bgrlex v₁ v₂) true) (fun h => isTrue (grlex_true_of_ble_grlex_true h))
+                                      (fun h => isFalse (grlex_false_of_ble_grlex_false h))
 
 end algebra
